$$
\begin{aligned}
\hat F(x)&=x\operatorname{EIJ}\operatorname{BIJ}\hat F(x)\\
&=x\exp\left(\frac{2\hat F(x)-\hat F^2(x)}{2-2\hat F(x)}\right)\\
G(\hat F(x))&=x\exp\left(\frac{2\hat F(x)-\hat F^2(x)}{2-2\hat F(x)}\right)-\hat F(x)\\
P(x)&=x\exp\left(\frac{F_0^2(x)-2F_0(x)}{2F_0(x)-2}\right)\\
F(x)&\equiv F_0(x)-\frac{G(F_0(x))}{G'(F_0(x))}\pmod{x^n}\\
&\equiv F_0(x)-\frac{P(x)-F_0(x)}{G'(F_0(x))}\pmod{x^n}\\
&\equiv F_0(x)-\frac{2P(x)-2F_0(x)}{P(x)\left(1+\frac1{(F_0(x)-1)^2}\right)-2}\pmod{x^n}\\
\end{aligned}
$$